Proof of equivocating_messages_exists theorem

theories/FullStates/protocol_states.v
@@ -182,4 +182,95 @@ Proof.
   repeat (split; try assumption). apply incl_tran with (get_messages sigma2); assumption.
 Qed.
 
+
+Definition two_senders := exists (v1 v2 : V), v1 <> v2.
+
+Lemma distinct_sender : two_senders -> forall v1 : V, exists v2 : V, v1 <> v2.
+Proof.
+  intros.
+  destruct H  as [v1' [v2' Hneq]].
+  destruct (v_eq_dec v1 v1') eqn:Heq.
+  - subst. exists v2'. assumption.
+  - exists v1'. assumption.
+Qed.
+
+Theorem not_extx_in_x : forall c v j j',
+  syntactic_state_inclusion j' j ->
+   ~ in_state (c, v, j) j'.
+Proof.
+  induction j'; intros;  unfold in_state; simpl; intro; try assumption.
+  destruct H0.
+  - inversion H0; subst; clear H0.
+    apply IHj'1; try apply incl_refl. apply H. left. reflexivity.
+  - apply IHj'2; try assumption.
+    intros msg Hin. apply H. right. assumption.
+Qed.
+
+Theorem equivocating_messages_exists :
+  two_senders ->
+  forall c v j,
+    protocol_state j ->
+    estimator j c ->
+    exists j' c',
+      j' in_Futures j /\
+      estimator j' c' /\
+      equivocating_messages (c, v, j) (c', v, j') = true.
+Proof.
+  intros H c v j H0 Hestj.
+  destruct (distinct_sender H v) as [v' Hneq].
+  exists (add_in_sorted_fn (c, v', j) j).
+  remember (add_in_sorted_fn (c, v', j) j) as j'.
+  destruct (estimator_total j') as [c' Hest].
+  exists c'.
+  split.
+  - split; try assumption.
+    split
+    ; try (subst; intros msg Hin; apply in_state_add_in_sorted_iff; right; assumption).
+    subst. constructor; try assumption; try apply incl_refl.
+    unfold fault_tolerance_condition. unfold fault_weight_state.
+    apply protocol_state_fault_tolerance in H0. unfold fault_tolerance_condition in H0.
+    apply Rle_trans with (fault_weight_state j); try assumption.
+    apply sum_weights_incl; try apply set_map_nodup.
+    unfold equivocating_senders. apply set_map_incl.
+    intros msg Hin.
+    apply filter_In in Hin. apply filter_In. destruct Hin.
+    apply in_state_add_in_sorted_iff in H1. destruct H1 as [Heq | Hin].
+    + subst. exfalso. unfold equivocating_message_state in H2.
+      rewrite existsb_exists in H2. destruct H2 as [msg [Hin Hequiv]].
+      apply in_state_add_in_sorted_iff in Hin.
+      destruct Hin as [Heq | Hin].
+      * subst. unfold equivocating_messages in Hequiv. rewrite eq_dec_if_true in Hequiv; try reflexivity.
+        inversion Hequiv.
+      * rewrite equivocating_messages_comm in Hequiv. rewrite non_equivocating_messages_extend in Hequiv
+        ; try assumption. inversion Hequiv.
+    + split; try assumption.
+      unfold equivocating_message_state in H2. apply existsb_exists in H2.
+      destruct H2 as [msg' [Hin' Hequiv]].
+      apply existsb_exists. exists msg'. split; try assumption.
+      apply in_state_add_in_sorted_iff in Hin'.
+      destruct Hin'; try assumption; subst.
+      exfalso. rewrite non_equivocating_messages_extend in Hequiv; try assumption. inversion Hequiv.
+  - split; try assumption.
+    unfold equivocating_messages.
+    rewrite eq_dec_if_false.
+    + rewrite eq_dec_if_true; try reflexivity.
+      rewrite andb_true_iff.
+      split; rewrite negb_true_iff
+      ; unfold in_state_fn; rewrite in_state_dec_if_false; try reflexivity
+      ; intro.
+      * subst. apply in_state_add_in_sorted_iff in H1.
+      { destruct H1.
+        - inversion H1. subst. apply Hneq. reflexivity.
+        - apply (not_extx_in_x c v j j); try assumption.
+          apply incl_refl.
+      }
+      * apply (not_extx_in_x c' v j' j); try assumption. subst.
+        intros msg Hin. apply in_state_add_in_sorted_iff. right. assumption.
+    + intro. inversion H1; subst; clear H1.
+      apply (not_extx_in_x c' v' j j); try apply incl_refl. rewrite H4 at 2.
+      apply in_state_add_in_sorted_iff. left. reflexivity.
+Qed.
+
+
+
 End Protocol_States.
